Source/test/proceduretest.bpl
@@ -2,16 +2,16 @@ procedure test() {
   var x: int, n: int where n >= 0, y: int;
   var q: int;
   havoc n;
-  x := -1;
-  x := increment(x);
+  x := 0;
   y := 0;
   while (x != n) {
       x := x + 1;
       //y := y + 1;
-      y := increment(y);
+      call y := increment(y);
   }
   assert (y >= n);
 }
 
-function {:define} increment(a:int) returns(int) { a + 1 }
-//axiom (forall i: int :: (increment(a) == a + 1));
+
+procedure increment(a: int) returns (b: int);
+  ensures b > a;
